\documentclass[UTF8]{report}
\usepackage{ctex}

\begin{document}
    \section*{29.}
        $$\begin{array}{l}
            M(s) = \sum_{x}e^{sx}p_X(x)\\
            = e^s \times \frac{1}{2} + e^{2s} \times \frac{1}{4} + e^{3s} \times \frac{1}{4}\\
        \end{array}$$

        所以：
        \begin{itemize}
            \item $E[X] = \frac{d}{ds}M(s)|_{s = 0} = \frac{7}{4}$
            \item $E[X^2] = \frac{d^2}{ds^2}M(s)|_{s = 0} = \frac{15}{4}$
            \item $E[X^3] = \frac{d^3}{ds^3}M(s)|_{s = 0} = \frac{37}{4}$
        \end{itemize}
    \section*{30.}
        标准正态分布$f_X(x) = \frac{1}{\sqrt{2\pi}}e^{\frac{-x^2}{2}}$，
        其矩母函数为
        $$\begin{array}{l}
            M(s) = \int_{-\infty}^{\infty}e^{sx}f_X(x)dx\\
            = \frac{1}{\sqrt{2\pi}}\int_{-\infty}^{\infty}e^{\frac{-x^2}{2} + sx}dx\\
            = \frac{1}{\sqrt{2\pi}}\int_{-\infty}^{\infty}e^{-\frac{x^2 - 2sx + s^2 - s^2}{2}}dx\\
            = \frac{e^{s^2}}{\sqrt{2\pi}}\int_{-\infty}^{\infty}e^{-\frac{(x - s)^2}{2}}dx\\
            = e^{s^2}
        \end{array}$$

        所以$E[X^3] = 0, E[X^4] = 12$。
    \section*{31.}
        $M(s) = \int_{0}^{\infty}\lambda e^{-\lambda x + sx}dx = \frac{-\lambda}{s - \lambda}$，
        所以$E[X^3] = \frac{6}{\lambda^4}, E[X^4] = \frac{24}{\lambda^5},\\ E[X^5] = \frac{120}{\lambda^6}$
\end{document}